## 1.
Suppose $T$ is linear. Let $u = (p,q,r), v=(x,y,z)$.
$$
T(u) = (2p-4q+3r+b,6p+cpqr) \\
T(v) = (2x-4y+3z+b,6x+cxyz)
$$

$$\begin{align*}
T(u+v) &= (2(p+x)-4(q+y)+3(r+z)+b,6(p+x)+c(p+x)(q+y)(r+z)) \\
\end{align*}$$

Since $T$ is linear, $T(u+v) = T(u) + T(v)$ and $T(\lambda u)=\lambda T(u)$.  
Thus, 
$$\begin{align*}
2(p+x)-4(q+y)+3(r+z)+b &= (2p-4q+3r+b) + (2x-4y+3z+b) \\
\end{align*}$$
Solving for $b$, we get $b=0$. 

$$\begin{align*}
\lambda(6p-cpqr) = 6\lambda p + c(\lambda p)(\lambda q)(\lambda r)
\end{align*}$$

Solving for $c$, we get $c=0$.

Suppose $b = c = 0$. Let $u = (p,q,r), v=(x,y,z)$.

$$
T(0) = 0
$$

$$\begin{align*}
T(u+v) &= (2(p+x)-4(q+y)+3(r+z),6(p+x)) \\
&= ((2p-4q+3r)+(2x-4y+3z),6p+6x) \\
&= T(u) + T(v)
\end{align*}$$

$$\begin{align*}
\lambda T(u) &= \lambda (2p-4q+3r,6p) \\
&= (2(\lambda p), -4(\lambda q) + 3(\lambda r), 6(\lambda p)) \\
&= T(\lambda u)
\end{align*}$$

Thus, $T$ is linear, as desired.


