## 1.

Let 
$$\begin{align*}
\alpha &= a + bi \\
\beta &= c + di \\
\end{align*}$$
where $\alpha, \beta \in \mathbb{C}.$

Then,
$$\begin{align*}
\alpha + \beta &= a + bi + c + di \\
&= c + di + a + bi \\
&= \beta + \alpha
\end{align*}$$

Thus, $\alpha + \beta = \beta + \alpha$
as desired.

## 2. 
Let 
$$\begin{align*}
\alpha &= a + bi \\
\beta &= c + di \\
\lambda &= e + fi \\
\end{align*}$$

where $\alpha, \beta, \lambda \in \mathbb{C}.$

Then, 
$$\begin{align*}
(\alpha + \beta) + \lambda &= (a + bi + c + di) + e + fi \\
&= a + bi + (c + di + e + fi) \\
&= \alpha + (\beta + \lambda)
\end{align*}$$

Thus,
$(\alpha + \beta) + \lambda = \alpha + (\beta + \lambda)$, as desired.

## 3.
Let 
$$\begin{align*}
\alpha &= a + bi \\
\beta &= c + di \\
\lambda &= e + fi \\
\end{align*}$$

where $\alpha, \beta, \lambda \in \mathbb{C}.$

Then, 
$$\begin{align*}
(\alpha\beta)\lambda &= [(a + bi)\cdot(c + di)]\cdot(e + fi) \\
&= [ac - bd + (ad + bc)i]\cdot(e + fi) \\
&= e\cdot(ac-bd) - f\cdot(ad+bc) + [f\cdot(ac - bd) + e\cdot(ad + bc)]i \\
&= a\cdot(ce - df) - b\cdot(cf + de) + [a\cdot(cf + de) + b\cdot(ce - df)]i \\
&= (a + bi)\cdot[(ce - df) + (cf + de)i] \\
&= (a + bi)\cdot[(c + di)\cdot(e + fi)] 

\end{align*}$$

Thus,
$(\alpha\beta)\lambda = \alpha(\beta\lambda)$, as desired.


## 4.
Let 
$$\begin{align*}
\alpha &= a + bi \\
\beta &= c + di \\
\lambda &= e + fi \\
\end{align*}$$

where $\alpha, \beta, \lambda \in \mathbb{C}.$

Then, 
$$\begin{align*}
\lambda(\alpha+\beta)&= (e+fi)(a+bi+c+di) \\
&= (e+fi)(a+bi) + (e+fi)(c+di) \\
&= \lambda\alpha + \lambda\beta
\end{align*}$$

Thus,
$\lambda(\alpha+\beta) = \lambda\alpha+\lambda\beta$, as desired.
